theories/Base.v
@@ -16,6 +16,28 @@ Proof using.
   exact tmp.
 Qed.
 
+Definition prod_dec {A B : Type} : (forall x y : A, {x = y} + {x <> y}) -> (forall x y : B, {x = y} + {x <> y}) ->
+  (forall x y : A * B, {x = y} + {x <> y}) := fun decA decB '(xa, xb) '(ya, yb) =>
+  match decA xa ya with
+  | right n => right (fun (f : (_, _) = (_, _)) => n (f_equal fst f))
+  | left ea =>
+    match decB xb yb with
+    | right n => right (fun (f : (_, _) = (_, _)) => n (f_equal snd f))
+    | left eb => left (f_equal2 pair ea eb)
+    end
+  end.
+
+Definition sigT_dec {A : Type} {B : A -> Type} : (forall x y : A, {x = y} + {x <> y}) -> (forall a (x y : B a), {x = y} + {x <> y}) ->
+  (forall x y : sigT B, {x = y} + {x <> y}) := fun decA decB '(existT _ xa xb) '(existT _ ya yb) =>
+  match decA xa ya with
+  | right n => right (fun f => n (EqdepFacts.eq_sigT_fst f))
+  | left ea =>
+    match decB _ (eq_rect _ B xb _ ea) yb with
+    | right n => right (fun f => n (eq_ind _ (fun v => eq_rect _ _ _ _ v = _) (EqdepFacts.eq_sigT_snd f) _ (Eqdep_dec.UIP_dec decA _ _)))
+    | left eb => left (eq_existT_curried ea eb)
+    end
+  end.
+
 Axiom ProofIrrelevance: forall (P: Prop) (p q: P), p = q.
 
 Lemma sig2T_eq_PI :
