theories/Translations/LustreOrderedToImp.v
@@ -2,103 +2,127 @@ From Reactive Require Import Base.
 From Reactive.Datatypes Require Ordered.
 From Reactive.Languages Require LustreOrdered Imp.
 
-Module Source := LustreOrdered.Lustre.
+Module Source := LustreOrdered.
 Module Target := Imp.
 
 
-Definition translate_const (c: LustreAst.const): Target.const :=
-  match c with
-  | LustreAst.CVoid => Target.CVoid
-  | LustreAst.CBool b => Target.CBool b
-  | LustreAst.CInt n => Target.CInt n
+Definition translate_type (ty: Source.type): Target.type :=
+  match ty with
+  | Source.Lustre.TVoid => Target.TVoid
+  | Source.Lustre.TBool => Target.TBool
+  | Source.Lustre.TInt => Target.TInt
   end.
 
-Definition translate_type (t: LustreAst.type): Target.type :=
-  match t with
-  | LustreAst.TVoid => Target.TVoid
-  | LustreAst.TBool => Target.TBool
-  | LustreAst.TInt => Target.TInt
+Definition translate_const {ty} (c: Source.const ty): Target.const (translate_type ty) :=
+  match c with
+  | Source.Lustre.CVoid => Target.CVoid
+  | Source.Lustre.CBool b => Target.CBool b
+  | Source.Lustre.CInt n => Target.CInt n
   end.
 
 Definition translate_binder (b: Source.binder): Target.binder :=
   (fst b, translate_type (snd b)).
 
-Definition translate_unop (op: LustreAst.unop): Target.unop :=
+Definition translate_unop {ty tout} (op: Source.unop ty tout): Target.unop (translate_type ty) (translate_type tout) :=
   match op with
-  | LustreAst.Uop_not => Target.Uop_not
-  | LustreAst.Uop_neg => Target.Uop_neg
+  | Source.Lustre.Uop_not => Target.Uop_not
+  | Source.Lustre.Uop_neg => Target.Uop_neg
   end.
 
-Definition translate_binop (op: LustreAst.binop): Target.binop :=
+Definition translate_binop {ty1 ty2 tout} (op: Source.binop ty1 ty2 tout):
+    match op with Source.Lustre.Bop_and | Source.Lustre.Bop_or => False | _ => True end ->
+    Target.binop (translate_type ty1) (translate_type ty2) (translate_type tout) :=
   match op with
-  | LustreAst.Bop_and => Target.Bop_and
-  | LustreAst.Bop_or => Target.Bop_or
-  | LustreAst.Bop_xor => Target.Bop_xor
-  | LustreAst.Bop_plus => Target.Bop_plus
-  | LustreAst.Bop_minus => Target.Bop_minus
-  | LustreAst.Bop_mult => Target.Bop_mult
-  | LustreAst.Bop_div => Target.Bop_div
-  | LustreAst.Bop_eq => Target.Bop_eq
-  | LustreAst.Bop_lt => Target.Bop_lt
-  | LustreAst.Bop_le => Target.Bop_le
-  | LustreAst.Bop_gt => Target.Bop_gt
-  | LustreAst.Bop_ge => Target.Bop_ge
+  | Source.Lustre.Bop_and => fun f => False_rect _ f
+  | Source.Lustre.Bop_or => fun f => False_rect _ f
+  | Source.Lustre.Bop_xor => fun _ => Target.Bop_xor
+  | Source.Lustre.Bop_plus => fun _ => Target.Bop_plus
+  | Source.Lustre.Bop_minus => fun _ => Target.Bop_minus
+  | Source.Lustre.Bop_mult => fun _ => Target.Bop_mult
+  | Source.Lustre.Bop_div => fun _ => Target.Bop_div
+  | Source.Lustre.Bop_eq => fun _ => Target.Bop_eq
+  | Source.Lustre.Bop_lt => fun _ => Target.Bop_lt
+  | Source.Lustre.Bop_le => fun _ => Target.Bop_le
+  | Source.Lustre.Bop_gt => fun _ => Target.Bop_gt
+  | Source.Lustre.Bop_ge => fun _ => Target.Bop_ge
   end.
 
-Fixpoint translate_value (v: Source.value): Target.value :=
+Fixpoint translate_value {ty} (v: Source.value ty): Target.value (translate_type ty) :=
   match v with
-  | Source.VConst c => Target.VConst (translate_const c)
-  | Source.VInput b => Target.VInput (translate_binder b)
-  | Source.VUnop op v => Target.VUnop (translate_unop op) (translate_value v)
-  | Source.VBinop op v1 v2 => Target.VBinop (translate_binop op) (translate_value v1) (translate_value v2)
-  | Source.VIfte v1 v2 v3 => Target.VIfte (translate_value v1) (translate_value v2) (translate_value v3)
+  | Source.Lustre.VConst c => Target.VConst (translate_const c)
+  | Source.Lustre.VInput b => Target.VInput (translate_binder b)
+  | Source.Lustre.VUnop op v => Target.VUnop (translate_unop op) (translate_value v)
+  | Source.Lustre.VBinop op v1 v2 =>
+      (match op in Source.Lustre.binop ty1 ty2 tout
+                return Target.value (translate_type ty1) -> Target.value (translate_type ty2) -> Target.value (translate_type tout) with
+      | Source.Lustre.Bop_and => fun v1 v2 =>
+          match v1 with
+          | Target.VConst (Target.CBool false) => Target.VConst (Target.CBool false)
+          | Target.VConst (Target.CBool true) => v2
+          | _ => Target.VBAnd v1 v2
+          end
+      | Source.Lustre.Bop_or => fun v1 v2 =>
+          match v1 with
+          | Target.VConst (Target.CBool false) => v2
+          | Target.VConst (Target.CBool true) => Target.VConst (Target.CBool true)
+          | _ => Target.VBOr v1 v2
+          end
+      | op => fun v1 v2 => Target.VBinop (translate_binop op I) v1 v2
+      end) (translate_value v1) (translate_value v2)
+  | Source.Lustre.VIfte v1 v2 v3 => Target.VIfte (translate_value v1) (translate_value v2) (translate_value v3)
   end.
 
-Fixpoint translate_exp (e: LustreAst.exp): Target.exp :=
+Fixpoint translate_exp {ty} (e: Source.exp ty): Target.exp (translate_type ty) :=
   match e with
-  | LustreAst.EConst c => Target.EConst (translate_const c)
-  | LustreAst.EInput b => Target.EInput (translate_binder b)
-  | LustreAst.EVar b => Target.EVar (translate_binder b)
-  | LustreAst.EUnop op e => Target.EUnop (translate_unop op) (translate_exp e)
-  | LustreAst.EBinop op e1 e2 => Target.EBinop (translate_binop op) (translate_exp e1) (translate_exp e2)
-  | LustreAst.EIfte e1 e2 e3 => Target.EIfte (translate_exp e1) (translate_exp e2) (translate_exp e3)
+  | Source.Lustre.EConst c => Target.EConst (translate_const c)
+  | Source.Lustre.EInput b => Target.EInput (translate_binder b)
+  | Source.Lustre.EVar b => Target.EVar (translate_binder b)
+  | Source.Lustre.EUnop op e => Target.EUnop (translate_unop op) (translate_exp e)
+  | Source.Lustre.EBinop op e1 e2 =>
+      (match op in Source.Lustre.binop ty1 ty2 tout return Source.exp ty1 -> Source.exp ty2 -> Target.exp (translate_type tout) with
+      | Source.Lustre.Bop_and => fun e1 e2 => Target.EBAnd (translate_exp e1) (translate_exp e2)
+      | Source.Lustre.Bop_or => fun e1 e2 => Target.EBOr (translate_exp e1) (translate_exp e2)
+      | op => fun e1 e2 => Target.EBinop (translate_binop op I) (translate_exp e1) (translate_exp e2)
+      end) e1 e2
+  | Source.Lustre.EIfte e1 e2 e3 => Target.EIfte (translate_exp e1) (translate_exp e2) (translate_exp e3)
   end.
 
-Definition translate_equation (eq: LustreAst.equation): Target.stmt :=
-  Target.SAssign (fst eq) (translate_exp (snd eq)).
+Definition translate_equation (eq: Source.equation): Target.stmt :=
+  Target.SAssign (fst eq, translate_type (projT1 (snd eq))) (translate_exp (projT2 (snd eq))).
 
 Definition translate_history (h: Source.history): Target.stack :=
-  Dict.map (fun x => translate_value (Stream.hd x)) h.
+  Dict.map (fun x => existT Target.value (translate_type (projT1 x)) (translate_value (Stream.hd (projT2 x)))) h.
 
-Definition translate_node_body (body: list LustreAst.equation): Target.stmt :=
+Definition translate_node_body (body: list Source.equation): Target.stmt :=
   fold_right (fun acc x => Target.SSeq x acc) Target.SNop (List.map translate_equation body).
 
-Lemma lustre_assignment_is_substmt (n: LustreOrdered.node_ordered) (name: ident) (exp: Source.exp):
-  let body := Source.n_body (LustreOrdered.node_ordered_is_node n) in
-  In (name, exp) body ->
-  Target.is_substmt (Target.SAssign name (translate_exp exp)) (translate_node_body body) = true.
+Lemma lustre_assignment_is_substmt (n: Source.node_ordered) (name: ident) (ty: Source.type) (exp: Source.exp ty):
+  let body := Source.Lustre.n_body (Source.node_ordered_is_node n) in
+  In (name, existT Source.exp ty exp) body ->
+  Target.is_substmt (Target.SAssign (name, translate_type ty) (translate_exp exp)) (translate_node_body body) = true.
 Proof.
   destruct n.
-  destruct node_ordered_is_node as [[]].
-  unfold Source.n_body in *.
+  destruct node_ordered_is_node as [].
+  unfold Source.Lustre.n_body in *.
   simpl in *.
   intros Hin.
   clear n_assigned_out n_inputs_equations n_no_einputs_in_other.
-  induction n_body as [ | (eq_left, eq_right) body IH ]; [ inversion Hin | ].
+  induction n_body as [ | (eq_left, (ty', eq_right)) body IH ]; [ inversion Hin | ].
   simpl.
   apply Bool.orb_true_intro.
   destruct Hin as [ Heq | Hin ].
-  - inversion Heq.
+  - injection Heq as eql eqt eqr.
+    subst.
+    apply Source.sig2T_eq_type in eqr.
     subst.
     right.
-    rewrite (PeanoNat.Nat.eqb_refl).
-    simpl.
+    rewrite PeanoNat.Nat.eqb_refl.
     rewrite Target.exp_eqb_refl.
     reflexivity.
   - left.
     apply IH.
     + intros i Hi.
-      pose proof (in_cons eq_left _ _ Hi) as H.
+      pose proof (in_cons (eq_left, ty') _ _ Hi) as H.
       apply n_assigned_vars_are_vars in H.
       assumption.
     + apply Ordered.cons in ordered.
@@ -106,11 +130,31 @@ Proof.
     + assumption.
 Qed.
 
-Definition translate_node (n: LustreOrdered.node_ordered): Target.method.
+Lemma in_map_fstsnd {A B} {C : B -> Type} (y: A * B) (xs: list (A * sigT C)):
+  In y (List.map (fun '(x, existT _ y _) => (x, y)) xs) ->
+    exists ys, In (fst y, existT C (snd y) ys) xs.
+Proof.
+  induction xs as [| x xs IHxs ].
+  { intros []. }
+
+  intros [ Heq | HIn ].
+  - subst.
+    destruct x as [ a [ b c ] ].
+    cbn in *.
+    exists c.
+    left.
+    reflexivity.
+  - destruct (IHxs HIn) as [ ys HIn' ].
+    exists ys.
+    right.
+    assumption.
+Qed.
+
+Definition translate_node (n: Source.node_ordered): Target.method.
 Proof.
   pose n as n'.
   destruct n.
-  destruct node_ordered_is_node as [[]].
+  destruct node_ordered_is_node as [].
   simpl in *.
 
   refine ({|
@@ -123,10 +167,10 @@ Proof.
     Target.m_body := translate_node_body n_body
   |}).
 
-  apply Sorted.in_map_fst in n_assigned_out as Hexp.
+  apply in_map_fstsnd in n_assigned_out as Hexp.
   destruct Hexp as [ exp Hexp ].
   exists (translate_exp exp).
-  replace n_body with (Source.n_body (LustreOrdered.node_ordered_is_node n')); [ | reflexivity ].
+  replace n_body with (Source.Lustre.n_body (Source.node_ordered_is_node n')); [ | reflexivity ].
   apply lustre_assignment_is_substmt.
   assumption.
 Defined.
@@ -134,23 +178,22 @@ Defined.
 
 (** Lemmas *)
 
-Lemma correctness_exp (e: Source.exp) (h: Source.history) (out: Source.value):
-  Source.sem_exp h e out ->
+Lemma correctness_exp (h: Source.history) {ty} (e: Source.exp ty) (out: Source.value ty):
+  Source.Lustre.sem_exp h e out ->
     Target.sem_exp (translate_history h) (translate_exp e) (translate_value out).
 Proof.
-  induction 1.
+  induction 1 as [| | | |h ty1 ty2 tout op e1 e2 v1 v2 H1 IH1 H2 IH2|].
 
   - (* EConst *)
     apply Target.SeConst.
 
   - (* EInput *)
-    apply Target.SeInput.
+    apply Target.SeInput with (b := translate_binder b).
 
   - (* EVar *)
-    apply Target.SeVar; simpl.
+    apply Target.SeVar with (b := translate_binder b); simpl.
 
-    pose (fun e => translate_const (Stream.hd e)) as f.
-    now apply Dict.maps_to_map with (f := fun x => translate_value (Stream.hd x)).
+    exact (Dict.maps_to_map _ _ _ _ H).
 
   - (* EUnop *)
     simpl.
@@ -160,109 +203,155 @@ Proof.
   - (* EBinop *)
     simpl.
 
-    apply Target.SeBinop; assumption.
+    destruct op; try solve [apply Target.SeBinop; assumption].
+    all: clear H1 H2.
+    all: remember (translate_history h) as th eqn:eqh.
+    all: remember (translate_exp e1) as te1 eqn:eqe1.
+    all: remember (translate_exp e2) as te2 eqn:eqe2.
+    all: remember (translate_value v1) as tv1 eqn:eqv1.
+    all: remember (translate_value v2) as tv2 eqn:eqv2.
+    all: clear h e1 e2 v1 v2 eqh eqe1 eqe2 eqv1 eqv2.
+    1,2: destruct (Target.value_inv tv1) as [ [ [ [ [ [
+      (c' & ->) | (b' & eq1 & ->) ] | (tin & op & v1' & ->) ] | (e & v1' & v2' & ->) ] | (e & v1' & v2' & ->) ] |
+      (ty1 & ty2 & op & v1' & v2' & ->) ] | (eb & et & ef & ->) ].
+    2: destruct b'; cbn in eq1; subst t.
+    4,5: rewrite (Eqdep_dec.UIP_dec Target.type_dec _ eq_refl) in *.
+    2-7: apply Target.SeBAndDefer; try assumption; discriminate.
+    3: destruct b'; cbn in eq1; subst t.
+    5,6: rewrite (Eqdep_dec.UIP_dec Target.type_dec _ eq_refl) in *.
+    3-8: apply Target.SeBOrDefer; try assumption; discriminate.
+    1,2: destruct (Target.const_inv c') as [ [ (e & [|] & ->) | (f & _) ] | (f & _) ]; try discriminate f.
+    1-4: rewrite (Eqdep_dec.UIP_dec Target.type_dec _ eq_refl) in *.
+    1: apply Target.SeBAndConstT; assumption.
+    1: apply Target.SeBAndConstF; assumption.
+    1: apply Target.SeBOrConstT; assumption.
+    1: apply Target.SeBOrConstF; assumption.
 
   - (* EIfte *)
     simpl.
     apply Target.SeIfte; assumption.
 Qed.
 
-Lemma sem_exp_without_useless_var (e: Source.exp) (h: Source.history) (name: ident) (v: Source.value):
-  Source.sem_exp h e v ->
-  ~ In name (LustreAst.var_of_exp e) ->
-    Source.sem_exp (Dict.remove name h) e v.
+Lemma sem_exp_without_useless_var (h: Source.history) (name: ident) {ty} (e: Source.exp ty) (v: Source.value ty):
+  Source.Lustre.sem_exp h e v ->
+  (forall tyv, ~ In (name, tyv) (Source.var_of_exp e)) ->
+    Source.Lustre.sem_exp (Dict.remove name h) e v.
 Proof.
   intros Hexp Hnin.
   revert v Hexp.
-  induction e as [ c | | (i, t) | op e IH | op e1 IH1 e2 IH2 | e1 IH1 e2 IH2 e3 IH3 ]; intros v Hexp.
+  induction e as [ ty c | (i, t) | (i, t) | ty tout op e IH | ty1 ty2 tout op e1 IH1 e2 IH2 | ty e1 IH1 e2 IH2 e3 IH3 ]; intros v Hexp.
   - inversion Hexp.
     subst.
-    apply Source.SeConst.
+    apply Source.sig2T_eq_type in H2, H3.
+    subst.
+    apply Source.Lustre.SeConst.
   - inversion Hexp.
     subst.
-    apply Source.SeInput.
+    apply Source.sig2T_eq_type in H4.
+    subst.
+    apply Source.Lustre.SeInput.
   - inversion Hexp.
     subst.
-    unfold LustreAst.var_of_exp in Hnin.
+    apply Source.sig2T_eq_type in H4.
+    subst.
+    unfold Source.var_of_exp in Hnin.
     simpl in Hnin.
-    apply Source.SeVar.
+    destruct b.
+    injection H3 as ->.
+    apply Source.Lustre.SeVar.
     simpl.
     apply Dict.maps_to_not_removed; [ assumption | ].
     intros Heq.
-    apply Hnin.
+    apply (Hnin t).
     left.
+    f_equal.
     assumption.
   - inversion Hexp.
     subst.
-    apply Source.SeUnop.
+    apply Source.sig2T_eq_type in H3, H4, H5.
+    apply Source.sig2T_eq_type in H3.
+    subst.
+    apply Source.Lustre.SeUnop.
     apply IH; assumption.
   - inversion Hexp.
     subst.
-    pose proof (Source.var_of_exp_not_in_binop e1 e2 name op) as [ H1' H2' ]; [ assumption | ].
-    apply Source.SeBinop.
+    apply Source.sig2T_eq_type in H4, H5, H6, H7.
+    do 2 apply Source.sig2T_eq_type in H4.
+    subst.
+    pose proof (Source.var_of_exp_not_in_binop e1 e2 name op) as tmp.
+    pose proof (fun ty => proj1 (tmp Hnin ty)) as H1'.
+    pose proof (fun ty => proj2 (tmp Hnin ty)) as H2'.
+    clear tmp.
+    apply Source.Lustre.SeBinop.
     + apply IH1; assumption.
     + apply IH2; assumption.
   - inversion Hexp.
     subst.
-    pose proof (Source.var_of_exp_not_in_ifte e1 e2 e3 name) as ( H1' & H2' & H3' ); [ assumption | ].
-    apply Source.SeIfte.
+    apply Source.sig2T_eq_type in H0, H1, H4.
+    subst.
+    pose proof (Source.var_of_exp_not_in_ifte e1 e2 e3 name) as tmp.
+    pose proof (fun ty => proj1 (tmp Hnin ty)) as H1'.
+    pose proof (fun ty => proj1 (proj2 (tmp Hnin ty))) as H2'.
+    pose proof (fun ty => proj2 (proj2 (tmp Hnin ty))) as H3'.
+    clear tmp.
+    apply Source.Lustre.SeIfte.
     + apply IH1; assumption.
     + apply IH2; assumption.
     + apply IH3; assumption.
 Qed.
 
-Definition evaluable_equations (s: Target.stack) (l: list LustreAst.equation): Prop :=
-  Forall (fun eq => exists v: Target.value, Target.sem_exp s (translate_exp (snd eq)) v) l.
+Definition evaluable_equations (s: Target.stack) (l: list Source.equation): Prop :=
+  Forall (fun '(name, existT _ ty eq) => exists v: Target.value _, Target.sem_exp s (translate_exp eq) v) l.
 
-Lemma ordered_equations_are_evaluable (h: Source.history) (l: list LustreAst.equation):
-  (Forall (fun eq =>
-      exists (v': Stream.t Source.value),
-      Dict.maps_to (fst eq) v' h /\ Source.sem_exp h (snd eq) (Stream.hd v')
+Lemma ordered_equations_are_evaluable (h: Source.history) (l: list Source.equation):
+  (Forall (fun '(name, existT _ ty eq) =>
+      exists (v': Stream.t (Source.value _)),
+      Dict.maps_to name (existT _ ty v') h /\ Source.Lustre.sem_exp h eq (Stream.hd v')
     ) l
   ) ->
-  Ordered.t (LustreOrdered.equations_to_dag l) -> evaluable_equations (translate_history h) l.
+  Ordered.t (Source.equations_to_dag l) -> evaluable_equations (translate_history h) l.
 Proof.
   intros Hhist Hord.
-  remember (LustreOrdered.equations_to_dag l) as dag.
+  remember (Source.equations_to_dag l) as dag.
   revert l Hhist Heqdag.
-  induction Hord as [ | x lx l' ]; intros l Hhist Heqdag.
+  induction Hord as [ | x lx l' ls ]; intros l Hhist Heqdag.
   - symmetry in Heqdag.
-    apply LustreOrdered.dag_nil in Heqdag.
+    apply Source.dag_nil in Heqdag.
     rewrite Heqdag.
     constructor.
   - destruct l as [ | eq l ]; [ constructor | ].
     simpl in Heqdag.
-    destruct eq as [ eq_left eq_right ].
+    destruct eq as [ eq_left [ ty eq_right ] ].
     inversion Heqdag.
     subst.
     constructor.
-    + assert (Forall (fun v => Dict.is_in v h) (LustreAst.var_of_exp eq_right)) as Hvars.
-      * apply LustreOrdered.Forall_impl_in with (P := fun y => exists ly, In (y, ly) (LustreOrdered.equations_to_dag l)); [ | assumption ].
+    + assert (Forall (fun v => Source.Lustre.in_history h v) (Source.var_of_exp eq_right)) as Hvars.
+      * apply Source.Forall_impl_in with (P := fun y => exists ly, In (y, ly) (Source.equations_to_dag l)); [ | assumption ].
         intros name Hin [ vars Hvars ].
         apply Forall_inv in Hhist as [ v' [ Hmaps Hsem ] ].
-        apply Source.sem_eval_exp in Hsem.
-        pose proof (Source.exp_evaluable_have_evaluable_vars _ _ _ Hsem) as H'.
+        apply Source.Lustre.sem_eval_exp in Hsem.
+        pose proof (Source.Lustre.exp_evaluable_have_evaluable_vars _ _ _ Hsem) as H'.
         apply Forall_forall with (x := name) in H'; assumption.
-      * pose proof (Source.exp_with_evaluable_vars_is_evaluable _ _ Hvars) as [ c Hc ].
+      * pose proof (Source.Lustre.exp_with_evaluable_vars_is_evaluable _ _ Hvars) as [ c Hc ].
         exists (translate_value c).
         apply correctness_exp.
-        apply Source.sem_eval_exp.
+        apply Source.Lustre.sem_eval_exp.
         assumption.
     + apply Forall_inv_tail in Hhist.
-      apply Forall_impl with (P := fun eq => exists v', Dict.maps_to (fst eq) v' h /\ Source.sem_exp h (snd eq) (Stream.hd v')); [ | assumption ].
-      intros (name, exp) [ v' [ Hmaps Hsem ] ].
+      refine (Forall_impl _ _ Hhist).
+      intros (name, (tyv, exp)) [ v' [ Hmaps Hsem ] ].
       exists (translate_value (Stream.hd v')).
       apply correctness_exp.
       assumption.
 Qed.
 
-Lemma translation_ordered_body (body: list LustreAst.equation) (h: Source.history):
-  Ordered.t (LustreOrdered.equations_to_dag body) ->
-  (Forall (fun eq =>
-      exists (v': Stream.t Source.value),
-      Dict.maps_to (fst eq) v' h /\ Source.sem_exp h (snd eq) (Stream.hd v')
+Lemma translation_ordered_body (body: list Source.equation) (h: Source.history):
+  Ordered.t (Source.equations_to_dag body) ->
+  (Forall (fun '(name, existT _ ty eq) =>
+      exists (v': Stream.t (Source.value _)),
+      Dict.maps_to name (existT _ _ v') h /\ Source.Lustre.sem_exp h eq (Stream.hd v')
   ) body ) ->
-  Forall (fun '(name, exp) => exists (v: Target.value), Target.sem_exp (translate_history h) (translate_exp exp) v) body.
+  Forall (fun '(name, existT _ ty exp) => exists (v: Target.value _), Target.sem_exp (translate_history h) (translate_exp exp) v) body.
 Proof.
   intros H Hhist.
   induction body; [ constructor | ].
@@ -270,6 +359,7 @@ Proof.
   - destruct a.
     apply ordered_equations_are_evaluable with (h := h) in H; [ | assumption ].
     apply Forall_inv in H.
+    destruct s.
     destruct H as [ c Hc ].
     simpl in *.
     exists c.
@@ -277,7 +367,8 @@ Proof.
   - destruct a.
     simpl in H.
     apply IHbody.
-    + apply Ordered.cons in H.
+    + destruct s.
+      apply Ordered.cons in H.
       assumption.
     + apply Forall_inv_tail in Hhist.
       assumption.
@@ -325,41 +416,41 @@ Proof.
         assumption.
 Qed.
 
-Lemma correctness_translation_equation (h: Source.history) (name: ident) (exp: Source.exp) (v: Stream.t Source.value):
-  Source.sem_exp h exp (Stream.hd v) ->
-  Dict.maps_to name v h ->
-  ~ In name (LustreAst.var_of_exp exp) ->
-  Target.sem_stmt (translate_history (Dict.remove name h)) (translate_equation (name, exp)) (translate_history h).
+Lemma correctness_translation_equation (h: Source.history) (name: ident) {ty} (exp: Source.exp ty) (v: Stream.t (Source.value _)):
+  Source.Lustre.sem_exp h exp (Stream.hd v) ->
+  Dict.maps_to name (existT _ ty v) h ->
+  (forall tyv, ~ In (name, tyv) (Source.var_of_exp exp)) ->
+  Target.sem_stmt (translate_history (Dict.remove name h)) (translate_equation (name, existT _ _ exp)) (translate_history h).
 Proof.
   intros Hexp Hmaps Hnin.
   unfold translate_equation.
   simpl.
-  rewrite Dict.remove_then_add_same_elt with (i := name) (x := translate_value (Stream.hd v)).
+  rewrite Dict.remove_then_add_same_elt with (i := name) (x := existT Target.value _ (translate_value (Stream.hd v))).
   - rewrite translation_history_element_removal.
     apply Target.SeAssign.
     apply correctness_exp.
     apply sem_exp_without_useless_var; assumption.
-  - apply Dict.maps_to_map with (f := fun x => translate_value (Stream.hd x)).
+  - apply Dict.maps_to_map with (f := fun x => existT Target.value _ (translate_value (Stream.hd (projT2 x)))) in Hmaps.
     assumption.
 Qed.
 
-Lemma correctness_node_under_history_assumptions (n: LustreOrdered.node_ordered) (h: Source.history):
-  (forall (i: ident), Dict.is_in i h <-> In i (map fst (Source.n_body (LustreOrdered.node_ordered_is_node n)))) ->
-  (Forall (fun eq =>
-      exists (v': Stream.t Source.value),
-      Dict.maps_to (fst eq) v' h /\ Source.sem_exp h (snd eq) (Stream.hd v')
-    ) (Source.n_body (LustreOrdered.node_ordered_is_node n))
+Lemma correctness_node_under_history_assumptions (n: Source.node_ordered) (h: Source.history):
+  (forall (i: ident), Dict.is_in i h <-> In i (map fst (Source.Lustre.n_body (Source.node_ordered_is_node n)))) ->
+  (Forall (fun '(n, existT _ ty eq) =>
+      exists (v': Stream.t (Source.value _)),
+      Dict.maps_to n (existT _ ty v') h /\ Source.Lustre.sem_exp h eq (Stream.hd v')
+    ) (Source.Lustre.n_body (Source.node_ordered_is_node n))
   ) ->
   Target.sem_stmt (Dict.empty _) (Target.m_body (translate_node n)) (translate_history h).
 Proof.
   intros Hhist Hsource.
   destruct n.
-  destruct node_ordered_is_node as [[]].
-  unfold Source.n_body in *.
+  destruct node_ordered_is_node as [].
+  unfold Source.Lustre.n_body in *.
   simpl in *.
   clear n_assigned_out n_inputs_equations n_no_einputs_in_other.
   revert h Hhist Hsource.
-  induction n_body as [ | (eq_left, eq_right) n_body IH ]; intros h Hhist Hsource.
+  induction n_body as [ | (eq_left, (ty, eq_right)) n_body IH ]; intros h Hhist Hsource.
   - simpl.
 
     assert (h = Dict.empty _).
@@ -380,10 +471,10 @@ Proof.
     apply Target.SeNop.
   - apply Ordered.cons in ordered as H.
     apply Ordered.cons in ordered as ordered_inner_body.
-    fold LustreOrdered.equations_to_dag in ordered_inner_body.
+    fold Source.equations_to_dag in ordered_inner_body.
     apply translation_ordered_body with (h := h) in ordered as Htrans; [ | assumption ].
 
-    assert (incl (map fst n_body) (map fst n_vars)) as Hincl.
+    assert (incl (map (fun '(n, existT _ ty _) => (n, ty)) n_body) n_vars) as Hincl.
     { intros x Hx.
       apply n_assigned_vars_are_vars.
       right.
@@ -402,7 +493,8 @@ Proof.
     2: { unfold translate_equation, hprev.
       simpl.
       apply correctness_translation_equation with (v := v'); [ assumption | assumption | ].
-      apply Ordered.var_not_need_itself in ordered.
+      intros tyv.
+      apply Ordered.var_not_need_itself with (b := tyv) in ordered.
       assumption. }
 
     apply IHprev.
@@ -430,7 +522,9 @@ Proof.
             exfalso.
             apply Ordered.vars_no_dups in ordered.
             apply ordered.
-            rewrite <- LustreOrdered.dag_names.
+            assert (tmp : forall l : list (ident * Source.type * list (ident * Source.type)), map (fun '(y, _, _) => y) l = map fst (map fst l))
+             by (clear; induction l as [|[[a b] c] tl IH]; [reflexivity|exact (f_equal _ IH)]).
+            rewrite tmp, <- Source.dag_names, map_map.
             assumption.
          ++ specialize (Hi2 (in_cons _ _ _ Hi)).
             destruct Hi2 as [ x Hx ].
@@ -438,8 +532,8 @@ Proof.
             exists x.
             assumption.
     * apply Forall_forall.
-      intros (i, x) Hin.
-      apply Forall_forall with (x := (i, x)) in Hsource_tail as Hix; [ | assumption ].
+      intros (i, (tyv, eq)) Hin.
+      apply (fun H => proj1 (Forall_forall _ _) H (i, existT _ tyv eq)) in Hsource_tail as Hix; [ | assumption ].
       destruct Hix as [ w' [ Hw'1 Hw'2 ] ].
       exists w'.
       split.
@@ -450,24 +544,47 @@ Proof.
             exfalso.
             apply Ordered.vars_no_dups in ordered.
             apply ordered.
-            rewrite <- LustreOrdered.dag_names.
+            assert (tmp : forall l : list (ident * Source.type * list (ident * Source.type)), map (fun '(y, _, _) => y) l = map fst (map fst l))
+             by (clear; induction l as [|[[a b] c] tl IH]; [reflexivity|exact (f_equal _ IH)]).
+            rewrite tmp, <- Source.dag_names, map_map.
             apply in_map with (f := fst) in Hin.
             assumption.
          ++ apply Dict.maps_to_not_removed; assumption.
       -- simpl in *.
          unfold hprev.
          apply sem_exp_without_useless_var; [ assumption | ].
-         apply Ordered.vars_coherence with (l := LustreOrdered.equations_to_dag n_body) (y := i) (lx := LustreAst.var_of_exp eq_right); [ assumption | ].
-         apply in_map with (f := fun '(i, x) => (i, LustreAst.var_of_exp x)) in Hin.
-         rewrite LustreOrdered.equations_to_dag_is_map.
+         intros tyv'.
+         apply (Ordered.vars_coherence _ i _ tyv _ _ _ ordered).
+         rewrite Source.equations_to_dag_is_map.
+         apply in_map with (f := fun '(i, existT _ ty e) => (i, ty, Source.var_of_exp e)) in Hin.
          assumption.
 Qed.
 
-Theorem correctness_node (n: LustreOrdered.node_ordered):
+Theorem correctness_node (n: Source.node_ordered):
   exists h: Source.history,
   Target.sem_stmt (Dict.empty _) (Target.m_body (translate_node n)) (translate_history h).
 Proof.
-  pose proof (LustreOrdered.minimal_history (Source.n_body (LustreOrdered.node_ordered_is_node n)) (LustreOrdered.ordered n)) as ( h & H1 & H2 ).
+  pose proof (Source.minimal_history (Source.Lustre.n_body (Source.node_ordered_is_node n)) (Source.ordered n)) as ( h & H1 & H2 ).
   exists h.
-  apply correctness_node_under_history_assumptions; assumption.
+  apply correctness_node_under_history_assumptions; [ clear H2 | assumption ].
+  intros i; specialize (H1 i).
+  cbn in H1.
+  split.
+  - intros [ [ ty s ] Hin ].
+    specialize (H1 ty).
+    rewrite Hin in H1.
+    apply proj1 in H1.
+    specialize (H1 eq_refl).
+    apply (in_map fst) in H1.
+    rewrite map_map in H1.
+    exact H1.
+  - intros Hin.
+    apply Sorted.in_map_fst in Hin.
+    destruct Hin as [ [ ty e ] Hin ].
+    apply (in_map Source.equation_dest) in Hin as Hin'.
+    apply H1 in Hin'.
+    destruct (Dict.find i h) as [ [ ty' s ] | ] eqn:Hfind; [ | contradiction Hin' ].
+    cbn in Hin'; subst ty'.
+    exists (existT _ ty s).
+    assumption.
 Qed.
