theories/Languages/Lustre.v
@@ -66,18 +66,18 @@ Inductive const : type -> Set :=
   | CInt: nat -> const TInt
 .
 Lemma const_inv {ty} (x: const ty) :
-  {eq : ty = _ & x = eq_rect _ const CVoid _ (eq_sym eq)} +
-  {eq : ty = _ & {b : bool & x = eq_rect _ const (CBool b) _ (eq_sym eq)}} +
-  {eq : ty = _ & {n : nat & x = eq_rect _ const (CInt n) _ (eq_sym eq)}}.
+  {eq : ty = _ & {b : bool | x = eq_rect _ const (CBool b) _ (eq_sym eq)}} +
+  {eq : ty = _ & {n : nat | x = eq_rect _ const (CInt n) _ (eq_sym eq)}} +
+  {exists (eq : ty = _), x = eq_rect _ const CVoid _ (eq_sym eq)}.
 Proof using.
-  destruct x as [|b|n]; [left; left|left; right|right]; exists eq_refl; [|exists b|exists n]; exact eq_refl.
+  destruct x as [|b|n]; [right|left; left|left; right]; exists eq_refl; [|exists b|exists n]; exact eq_refl.
 Qed.
 Lemma const_dec {ty} (x y: const ty) : {x = y} + {x <> y}.
 Proof.
-  destruct x.
-  all: destruct (const_inv y) as [[[eq' ->]|[eq' [b' ->]]]|[eq' [n' ->]]].
-  all: try discriminate.
-  1: left.
+  destruct x as [ | b | n ].
+  all: destruct (const_inv y) as [[[eq' [b' ->]]|[eq' [n' ->]]]|H].
+  all: try discriminate; try solve [right; destruct H as [f _]; discriminate f].
+  1: left; destruct H as [eq' ->].
   2: destruct (Bool.bool_dec b b') as [eq|ne]; [left|right].
   4: destruct (PeanoNat.Nat.eq_dec n n') as [eq|ne]; [left|right].
   all: rewrite !(Eqdep_dec.UIP_dec type_dec _ eq_refl); cbn; try intros [=f]; auto.
@@ -95,19 +95,23 @@ Inductive unop: type -> type -> Set :=
 .
 
 Lemma unop_inv {ty tout} (x: unop ty tout) :
-  {eq1 : ty = TInt & {eq2 : tout = TInt & x = eq_rect _ (unop _) (eq_rect _ (fun ty => unop ty _) Uop_not _ (eq_sym eq1)) _ (eq_sym eq2)}} +
-  {eq1 : ty = TInt & {eq2 : tout = TInt & x = eq_rect _ (unop _) (eq_rect _ (fun ty => unop ty _) Uop_neg _ (eq_sym eq1)) _ (eq_sym eq2)}}.
+  {exists (eq1 : ty = TInt) (eq2 : tout = TInt), x = eq_rect _ (unop _) (eq_rect _ (fun ty => unop ty _) Uop_not _ (eq_sym eq1)) _ (eq_sym eq2)} +
+  {exists (eq1 : ty = TInt) (eq2 : tout = TInt), x = eq_rect _ (unop _) (eq_rect _ (fun ty => unop ty _) Uop_neg _ (eq_sym eq1)) _ (eq_sym eq2)}.
 Proof using.
   destruct x; [left|right]; exists eq_refl, eq_refl; exact eq_refl.
 Qed.
 Lemma unop_dec {ty tout} (x y: unop ty tout) : {x = y} + {x <> y}.
 Proof.
-  destruct (unop_inv x) as [[eq1 [eq2 ->]]|[eq1 [eq2 ->]]].
-  all: destruct (unop_inv y) as [[-> [-> ->]]|[-> [-> ->]]].
+  destruct (unop_inv x) as [H1|H1].
+  all: destruct (unop_inv y) as [H2|H2].
+  1,4: left.
+  3,4: right.
+  all: destruct H1 as [eq1 [eq2 ->]].
+  all: destruct H2 as [-> [-> ->]].
   all: rewrite !(Eqdep_dec.UIP_dec type_dec _ eq_refl); cbn.
   all: rewrite !(Eqdep_dec.UIP_dec type_dec _ eq_refl); cbn.
-  1,4: left; reflexivity.
-  all: right; discriminate.
+  1-2: reflexivity.
+  all: discriminate.
 Qed.
 
 (** A binary operator
@@ -136,18 +140,18 @@ Inductive binop: type -> type -> type -> Set :=
 .
 
 Lemma binop_inv {ty1 ty2 tout} (x: binop ty1 ty2 tout) :
-  {eq1 : ty1 = _ & {eq2 : ty2 = _ & {eqo : tout = _ & x = eq_rect _ (binop _ _) (eq_rect _ (fun ty => binop _ ty _) (eq_rect _ (fun ty => binop ty _ _) Bop_and _ (eq_sym eq1)) _ (eq_sym eq2)) _ (eq_sym eqo)}}} +
-  {eq1 : ty1 = _ & {eq2 : ty2 = _ & {eqo : tout = _ & x = eq_rect _ (binop _ _) (eq_rect _ (fun ty => binop _ ty _) (eq_rect _ (fun ty => binop ty _ _) Bop_or _ (eq_sym eq1)) _ (eq_sym eq2)) _ (eq_sym eqo)}}} +
-  {eq1 : ty1 = _ & {eq2 : ty2 = _ & {eqo : tout = _ & x = eq_rect _ (binop _ _) (eq_rect _ (fun ty => binop _ ty _) (eq_rect _ (fun ty => binop ty _ _) Bop_xor _ (eq_sym eq1)) _ (eq_sym eq2)) _ (eq_sym eqo)}}} +
-  {eq1 : ty1 = _ & {eq2 : ty2 = _ & {eqo : tout = _ & x = eq_rect _ (binop _ _) (eq_rect _ (fun ty => binop _ ty _) (eq_rect _ (fun ty => binop ty _ _) Bop_plus _ (eq_sym eq1)) _ (eq_sym eq2)) _ (eq_sym eqo)}}} +
-  {eq1 : ty1 = _ & {eq2 : ty2 = _ & {eqo : tout = _ & x = eq_rect _ (binop _ _) (eq_rect _ (fun ty => binop _ ty _) (eq_rect _ (fun ty => binop ty _ _) Bop_minus _ (eq_sym eq1)) _ (eq_sym eq2)) _ (eq_sym eqo)}}} +
-  {eq1 : ty1 = _ & {eq2 : ty2 = _ & {eqo : tout = _ & x = eq_rect _ (binop _ _) (eq_rect _ (fun ty => binop _ ty _) (eq_rect _ (fun ty => binop ty _ _) Bop_mult _ (eq_sym eq1)) _ (eq_sym eq2)) _ (eq_sym eqo)}}} +
-  {eq1 : ty1 = _ & {eq2 : ty2 = _ & {eqo : tout = _ & x = eq_rect _ (binop _ _) (eq_rect _ (fun ty => binop _ ty _) (eq_rect _ (fun ty => binop ty _ _) Bop_div _ (eq_sym eq1)) _ (eq_sym eq2)) _ (eq_sym eqo)}}} +
-  {eq1 : ty1 = _ & {eq2 : ty2 = _ & {eqo : tout = _ & x = eq_rect _ (binop _ _) (eq_rect _ (fun ty => binop _ ty _) (eq_rect _ (fun ty => binop ty _ _) Bop_eq _ (eq_sym eq1)) _ (eq_sym eq2)) _ (eq_sym eqo)}}} +
-  {eq1 : ty1 = _ & {eq2 : ty2 = _ & {eqo : tout = _ & x = eq_rect _ (binop _ _) (eq_rect _ (fun ty => binop _ ty _) (eq_rect _ (fun ty => binop ty _ _) Bop_le _ (eq_sym eq1)) _ (eq_sym eq2)) _ (eq_sym eqo)}}} +
-  {eq1 : ty1 = _ & {eq2 : ty2 = _ & {eqo : tout = _ & x = eq_rect _ (binop _ _) (eq_rect _ (fun ty => binop _ ty _) (eq_rect _ (fun ty => binop ty _ _) Bop_lt _ (eq_sym eq1)) _ (eq_sym eq2)) _ (eq_sym eqo)}}} +
-  {eq1 : ty1 = _ & {eq2 : ty2 = _ & {eqo : tout = _ & x = eq_rect _ (binop _ _) (eq_rect _ (fun ty => binop _ ty _) (eq_rect _ (fun ty => binop ty _ _) Bop_ge _ (eq_sym eq1)) _ (eq_sym eq2)) _ (eq_sym eqo)}}} +
-  {eq1 : ty1 = _ & {eq2 : ty2 = _ & {eqo : tout = _ & x = eq_rect _ (binop _ _) (eq_rect _ (fun ty => binop _ ty _) (eq_rect _ (fun ty => binop ty _ _) Bop_gt _ (eq_sym eq1)) _ (eq_sym eq2)) _ (eq_sym eqo)}}}.
+  {exists (eq1 : ty1 = _) (eq2 : ty2 = _) (eqo : tout = _), x = eq_rect _ (binop _ _) (eq_rect _ (fun ty => binop _ ty _) (eq_rect _ (fun ty => binop ty _ _) Bop_and _ (eq_sym eq1)) _ (eq_sym eq2)) _ (eq_sym eqo)} +
+  {exists (eq1 : ty1 = _) (eq2 : ty2 = _) (eqo : tout = _), x = eq_rect _ (binop _ _) (eq_rect _ (fun ty => binop _ ty _) (eq_rect _ (fun ty => binop ty _ _) Bop_or _ (eq_sym eq1)) _ (eq_sym eq2)) _ (eq_sym eqo)} +
+  {exists (eq1 : ty1 = _) (eq2 : ty2 = _) (eqo : tout = _), x = eq_rect _ (binop _ _) (eq_rect _ (fun ty => binop _ ty _) (eq_rect _ (fun ty => binop ty _ _) Bop_xor _ (eq_sym eq1)) _ (eq_sym eq2)) _ (eq_sym eqo)} +
+  {exists (eq1 : ty1 = _) (eq2 : ty2 = _) (eqo : tout = _), x = eq_rect _ (binop _ _) (eq_rect _ (fun ty => binop _ ty _) (eq_rect _ (fun ty => binop ty _ _) Bop_plus _ (eq_sym eq1)) _ (eq_sym eq2)) _ (eq_sym eqo)} +
+  {exists (eq1 : ty1 = _) (eq2 : ty2 = _) (eqo : tout = _), x = eq_rect _ (binop _ _) (eq_rect _ (fun ty => binop _ ty _) (eq_rect _ (fun ty => binop ty _ _) Bop_minus _ (eq_sym eq1)) _ (eq_sym eq2)) _ (eq_sym eqo)} +
+  {exists (eq1 : ty1 = _) (eq2 : ty2 = _) (eqo : tout = _), x = eq_rect _ (binop _ _) (eq_rect _ (fun ty => binop _ ty _) (eq_rect _ (fun ty => binop ty _ _) Bop_mult _ (eq_sym eq1)) _ (eq_sym eq2)) _ (eq_sym eqo)} +
+  {exists (eq1 : ty1 = _) (eq2 : ty2 = _) (eqo : tout = _), x = eq_rect _ (binop _ _) (eq_rect _ (fun ty => binop _ ty _) (eq_rect _ (fun ty => binop ty _ _) Bop_div _ (eq_sym eq1)) _ (eq_sym eq2)) _ (eq_sym eqo)} +
+  {exists (eq1 : ty1 = _) (eq2 : ty2 = _) (eqo : tout = _), x = eq_rect _ (binop _ _) (eq_rect _ (fun ty => binop _ ty _) (eq_rect _ (fun ty => binop ty _ _) Bop_eq _ (eq_sym eq1)) _ (eq_sym eq2)) _ (eq_sym eqo)} +
+  {exists (eq1 : ty1 = _) (eq2 : ty2 = _) (eqo : tout = _), x = eq_rect _ (binop _ _) (eq_rect _ (fun ty => binop _ ty _) (eq_rect _ (fun ty => binop ty _ _) Bop_le _ (eq_sym eq1)) _ (eq_sym eq2)) _ (eq_sym eqo)} +
+  {exists (eq1 : ty1 = _) (eq2 : ty2 = _) (eqo : tout = _), x = eq_rect _ (binop _ _) (eq_rect _ (fun ty => binop _ ty _) (eq_rect _ (fun ty => binop ty _ _) Bop_lt _ (eq_sym eq1)) _ (eq_sym eq2)) _ (eq_sym eqo)} +
+  {exists (eq1 : ty1 = _) (eq2 : ty2 = _) (eqo : tout = _), x = eq_rect _ (binop _ _) (eq_rect _ (fun ty => binop _ ty _) (eq_rect _ (fun ty => binop ty _ _) Bop_ge _ (eq_sym eq1)) _ (eq_sym eq2)) _ (eq_sym eqo)} +
+  {exists (eq1 : ty1 = _) (eq2 : ty2 = _) (eqo : tout = _), x = eq_rect _ (binop _ _) (eq_rect _ (fun ty => binop _ ty _) (eq_rect _ (fun ty => binop ty _ _) Bop_gt _ (eq_sym eq1)) _ (eq_sym eq2)) _ (eq_sym eqo)}.
 Proof using.
   destruct x.
   1-11: left.
@@ -166,77 +170,76 @@ Proof using.
 Qed.
 Lemma binop_dec {ty1 ty2 tout} (x y: binop ty1 ty2 tout) : {x = y} + {x <> y}.
 Proof.
-  pose proof (binop_inv x) as H.
-  repeat destruct H as [ H | [eq1 [eq2 [eq3 ->]]] ].
-  1: destruct H as [eq1 [eq2 [eq3 ->]]].
+  pose proof (binop_inv x) as H1.
+  repeat destruct H1 as [ H1 | H1 ].
   all: pose proof (binop_inv y) as H.
-  12: destruct H as [f|[-> [-> [-> ->]]]]; [right|left].
+  12: destruct H as [f|H]; [right|left]; destruct H1 as [eq1 [eq2 [eq3 ->]]]; [|destruct H as [-> [-> [-> ->]]]].
   13: do 3 (rewrite (Eqdep_dec.UIP_dec type_dec _ eq_refl); cbn); reflexivity.
-  1-11: destruct H as [H|[-> [-> [-> f]]]]; [|
-    right; try discriminate; intros <-;
-    repeat (rewrite (Eqdep_dec.UIP_dec type_dec _ eq_refl) in f; cbn in f); try discriminate
+  1-11: destruct H as [H|f]; [|
+    right; destruct H1 as [eq1 [eq2 [eq3 ->]]], f as [-> [-> [-> f]]]; try discriminate; intros <-;
+    repeat (rewrite (Eqdep_dec.UIP_dec type_dec _ eq_refl) in f; cbn in f); discriminate
   ].
-  11: destruct H as [f|[-> [-> [-> ->]]]]; [right|left].
+  11: destruct H as [f|H]; [right|left]; destruct H1 as [eq1 [eq2 [eq3 ->]]]; [|destruct H as [-> [-> [-> ->]]]].
   12: do 3 (rewrite (Eqdep_dec.UIP_dec type_dec _ eq_refl); cbn); reflexivity.
-  1-10: destruct H as [H|[-> [-> [-> f]]]]; [|
-    right; try discriminate; intros <-;
-    repeat (rewrite (Eqdep_dec.UIP_dec type_dec _ eq_refl) in f; cbn in f); try discriminate
+  1-10: destruct H as [H|f]; [|
+    right; destruct H1 as [eq1 [eq2 [eq3 ->]]], f as [-> [-> [-> f]]]; try discriminate; intros <-;
+    repeat (rewrite (Eqdep_dec.UIP_dec type_dec _ eq_refl) in f; cbn in f); discriminate
   ].
-  10: destruct H as [f|[-> [-> [-> ->]]]]; [right|left].
+  10: destruct H as [f|H]; [right|left]; destruct H1 as [eq1 [eq2 [eq3 ->]]]; [|destruct H as [-> [-> [-> ->]]]].
   11: do 3 (rewrite (Eqdep_dec.UIP_dec type_dec _ eq_refl); cbn); reflexivity.
-  1-9: destruct H as [H|[-> [-> [-> f]]]]; [|
-    right; try discriminate; intros <-;
-    repeat (rewrite (Eqdep_dec.UIP_dec type_dec _ eq_refl) in f; cbn in f); try discriminate
+  1-9: destruct H as [H|f]; [|
+    right; destruct H1 as [eq1 [eq2 [eq3 ->]]], f as [-> [-> [-> f]]]; try discriminate; intros <-;
+    repeat (rewrite (Eqdep_dec.UIP_dec type_dec _ eq_refl) in f; cbn in f); discriminate
   ].
-  9: destruct H as [f|[-> [-> [-> ->]]]]; [right|left].
+  9: destruct H as [f|H]; [right|left]; destruct H1 as [eq1 [eq2 [eq3 ->]]]; [|destruct H as [-> [-> [-> ->]]]].
   10: do 3 (rewrite (Eqdep_dec.UIP_dec type_dec _ eq_refl); cbn); reflexivity.
-  1-8: destruct H as [H|[-> [-> [-> f]]]]; [|
-    right; try discriminate; intros <-;
-    repeat (rewrite (Eqdep_dec.UIP_dec type_dec _ eq_refl) in f; cbn in f); try discriminate
+  1-8: destruct H as [H|f]; [|
+    right; destruct H1 as [eq1 [eq2 [eq3 ->]]], f as [-> [-> [-> f]]]; try discriminate; intros <-;
+    repeat (rewrite (Eqdep_dec.UIP_dec type_dec _ eq_refl) in f; cbn in f); discriminate
   ].
-  8: destruct H as [f|[-> [-> [-> ->]]]]; [right|left].
+  8: destruct H as [f|H]; [right|left]; destruct H1 as [eq1 [eq2 [eq3 ->]]]; [|destruct H as [-> [-> [-> ->]]]].
   9: do 3 (rewrite (Eqdep_dec.UIP_dec type_dec _ eq_refl); cbn); reflexivity.
-  1-7: destruct H as [H|[-> [-> [-> f]]]]; [|
-    right; try discriminate; intros <-;
-    repeat (rewrite (Eqdep_dec.UIP_dec type_dec _ eq_refl) in f; cbn in f); try discriminate
+  1-7: destruct H as [H|f]; [|
+    right; destruct H1 as [eq1 [eq2 [eq3 ->]]], f as [-> [-> [-> f]]]; try discriminate; intros <-;
+    repeat (rewrite (Eqdep_dec.UIP_dec type_dec _ eq_refl) in f; cbn in f); discriminate
   ].
-  7: destruct H as [f|[-> [-> [-> ->]]]]; [right|left].
+  7: destruct H as [f|H]; [right|left]; destruct H1 as [eq1 [eq2 [eq3 ->]]]; [|destruct H as [-> [-> [-> ->]]]].
   8: do 3 (rewrite (Eqdep_dec.UIP_dec type_dec _ eq_refl); cbn); reflexivity.
-  1-6: destruct H as [H|[-> [-> [-> f]]]]; [|
-    right; try discriminate; intros <-;
-    repeat (rewrite (Eqdep_dec.UIP_dec type_dec _ eq_refl) in f; cbn in f); try discriminate
+  1-6: destruct H as [H|f]; [|
+    right; destruct H1 as [eq1 [eq2 [eq3 ->]]], f as [-> [-> [-> f]]]; try discriminate; intros <-;
+    repeat (rewrite (Eqdep_dec.UIP_dec type_dec _ eq_refl) in f; cbn in f); discriminate
   ].
-  6: destruct H as [f|[-> [-> [-> ->]]]]; [right|left].
+  6: destruct H as [f|H]; [right|left]; destruct H1 as [eq1 [eq2 [eq3 ->]]]; [|destruct H as [-> [-> [-> ->]]]].
   7: do 3 (rewrite (Eqdep_dec.UIP_dec type_dec _ eq_refl); cbn); reflexivity.
-  1-5: destruct H as [H|[-> [-> [-> f]]]]; [|
-    right; try discriminate; intros <-;
-    repeat (rewrite (Eqdep_dec.UIP_dec type_dec _ eq_refl) in f; cbn in f); try discriminate
+  1-5: destruct H as [H|f]; [|
+    right; destruct H1 as [eq1 [eq2 [eq3 ->]]], f as [-> [-> [-> f]]]; try discriminate; intros <-;
+    repeat (rewrite (Eqdep_dec.UIP_dec type_dec _ eq_refl) in f; cbn in f); discriminate
   ].
-  5: destruct H as [f|[-> [-> [-> ->]]]]; [right|left].
+  5: destruct H as [f|H]; [right|left]; destruct H1 as [eq1 [eq2 [eq3 ->]]]; [|destruct H as [-> [-> [-> ->]]]].
   6: do 3 (rewrite (Eqdep_dec.UIP_dec type_dec _ eq_refl); cbn); reflexivity.
-  1-4: destruct H as [H|[-> [-> [-> f]]]]; [|
-    right; try discriminate; intros <-;
-    repeat (rewrite (Eqdep_dec.UIP_dec type_dec _ eq_refl) in f; cbn in f); try discriminate
+  1-4: destruct H as [H|f]; [|
+    right; destruct H1 as [eq1 [eq2 [eq3 ->]]], f as [-> [-> [-> f]]]; try discriminate; intros <-;
+    repeat (rewrite (Eqdep_dec.UIP_dec type_dec _ eq_refl) in f; cbn in f); discriminate
   ].
-  4: destruct H as [f|[-> [-> [-> ->]]]]; [right|left].
+  4: destruct H as [f|H]; [right|left]; destruct H1 as [eq1 [eq2 [eq3 ->]]]; [|destruct H as [-> [-> [-> ->]]]].
   5: do 3 (rewrite (Eqdep_dec.UIP_dec type_dec _ eq_refl); cbn); reflexivity.
-  1-3: destruct H as [H|[-> [-> [-> f]]]]; [|
-    right; try discriminate; intros <-;
-    repeat (rewrite (Eqdep_dec.UIP_dec type_dec _ eq_refl) in f; cbn in f); try discriminate
+  1-3: destruct H as [H|f]; [|
+    right; destruct H1 as [eq1 [eq2 [eq3 ->]]], f as [-> [-> [-> f]]]; try discriminate; intros <-;
+    repeat (rewrite (Eqdep_dec.UIP_dec type_dec _ eq_refl) in f; cbn in f); discriminate
   ].
-  3: destruct H as [f|[-> [-> [-> ->]]]]; [right|left].
+  3: destruct H as [f|H]; [right|left]; destruct H1 as [eq1 [eq2 [eq3 ->]]]; [|destruct H as [-> [-> [-> ->]]]].
   4: do 3 (rewrite (Eqdep_dec.UIP_dec type_dec _ eq_refl); cbn); reflexivity.
-  1-2: destruct H as [H|[-> [-> [-> f]]]]; [|
-    right; try discriminate; intros <-;
-    repeat (rewrite (Eqdep_dec.UIP_dec type_dec _ eq_refl) in f; cbn in f); try discriminate
+  1-2: destruct H as [H|f]; [|
+    right; destruct H1 as [eq1 [eq2 [eq3 ->]]], f as [-> [-> [-> f]]]; try discriminate; intros <-;
+    repeat (rewrite (Eqdep_dec.UIP_dec type_dec _ eq_refl) in f; cbn in f); discriminate
   ].
-  2: destruct H as [f|[-> [-> [-> ->]]]]; [right|left].
+  2: destruct H as [f|H]; [right|left]; destruct H1 as [eq1 [eq2 [eq3 ->]]]; [|destruct H as [-> [-> [-> ->]]]].
   3: do 3 (rewrite (Eqdep_dec.UIP_dec type_dec _ eq_refl); cbn); reflexivity.
-  1: destruct H as [H|[-> [-> [-> f]]]]; [|
-    right; try discriminate; intros <-;
-    repeat (rewrite (Eqdep_dec.UIP_dec type_dec _ eq_refl) in f; cbn in f); try discriminate
+  1: destruct H as [H|f]; [|
+    right; destruct H1 as [eq1 [eq2 [eq3 ->]]], f as [-> [-> [-> f]]]; try discriminate; intros <-;
+    repeat (rewrite (Eqdep_dec.UIP_dec type_dec _ eq_refl) in f; cbn in f); discriminate
   ].
-  1: destruct H as [-> [-> [-> ->]]]; left.
+  1: left; destruct H1 as [eq1 [eq2 [eq3 ->]]], H as [-> [-> [-> ->]]].
   1: do 3 (rewrite (Eqdep_dec.UIP_dec type_dec _ eq_refl); cbn); reflexivity.
   all: subst; cbn; intros <-; repeat (destruct f as [f|[? [? [? f]]]]; [|try discriminate]).
   all: try solve [repeat (rewrite (Eqdep_dec.UIP_dec type_dec _ eq_refl) in f; cbn in f); discriminate f].
@@ -254,12 +257,12 @@ Inductive exp : type -> Set :=
 .
 
 Lemma exp_inv {ty} (x: exp ty) :
-  {c : const ty & x = EConst c} +
-  {b & {eq : ty = _ & x = eq_rect _ exp (EInput b) _ (eq_sym eq)}} +
-  {b & {eq : ty = _ & x = eq_rect _ exp (EVar b) _ (eq_sym eq)}} +
-  {tin : type & {op : unop tin ty & {e : exp tin & x = EUnop op e}}} +
-  {ty1 : type & {ty2 : type & {op : binop ty1 ty2 ty & {e1 : exp ty1 & {e2 : exp ty2 & x = EBinop op e1 e2}}}}} +
-  {eb : exp TBool & {et : exp ty & {ef : exp ty & x = EIfte eb et ef}}}.
+  {c : const ty | x = EConst c} +
+  {b | exists (eq : ty = _), x = eq_rect _ exp (EInput b) _ (eq_sym eq)} +
+  {b | exists (eq : ty = _), x = eq_rect _ exp (EVar b) _ (eq_sym eq)} +
+  {tin : type & {op : unop tin ty & {e : exp tin | x = EUnop op e}}} +
+  {ty1 : type & {ty2 : type & {op : binop ty1 ty2 ty & {e1 : exp ty1 & {e2 : exp ty2 | x = EBinop op e1 e2}}}}} +
+  {eb : exp TBool & {et : exp ty & {ef : exp ty | x = EIfte eb et ef}}}.
 Proof using.
   destruct x.
   1-5: left.
@@ -276,31 +279,31 @@ Proof.
   revert e2.
   induction e1 as [ ty c | b | b | tin tout op e1 IH | ty1 ty2 tout op e11 IH1 e12 IH2 | ty eb1 IHb et1 IHt ef1 IHf ].
   - intros e2; destruct (exp_inv e2) as [ [ [ [ [
-      (c' & ->) | (b' & eq1 & ->) ] | (b' & eq1 & ->) ] | (tin & op & e1' & ->) ] | (ty1 & ty2 & op & e1' & e2' & ->) ] | (eb & et & ef & ->) ].
+      (c' & ->) | (b' & H) ] | (b' & H) ] | (tin & op & e1' & ->) ] | (ty1 & ty2 & op & e1' & e2' & ->) ] | (eb & et & ef & ->) ].
     1: destruct (const_dec c c') as [e|n]; [left; exact (f_equal _ e)|right; intros [=f]; apply sig2T_eq_type in f; exact (n f)].
-    all: right; subst; discriminate.
+    all: right; try destruct H as [eq1 ->]; subst; discriminate.
   - intros e2; destruct (exp_inv e2) as [ [ [ [ [
-      (c' & ->) | (b' & eq1 & ->) ] | (b' & eq1 & ->) ] | (tin & op & e1' & ->) ] | (ty1 & ty2 & op & e1' & e2' & ->) ] | (eb & et & ef & ->) ].
-    3: right; destruct b, b'; cbn in eq1; subst; discriminate.
+      (c' & ->) | (b' & H) ] | (b' & H) ] | (tin & op & e1' & ->) ] | (ty1 & ty2 & op & e1' & e2' & ->) ] | (eb & et & ef & ->) ].
+    3: right; destruct H as [eq1 ->]; destruct b, b'; cbn in eq1; subst; discriminate.
     1,3-5: right; subst; discriminate.
-    destruct b as [n1 ty1], b' as [n2 ty2]; cbn in eq1; subst ty2.
-    destruct (PeanoNat.Nat.eq_dec n1 n2) as [<-|ne]; [left; reflexivity|right; cbn; intros [=f]; exact (ne f)].
+    destruct b as [n1 ty1], b' as [n2 ty2].
+    destruct (PeanoNat.Nat.eq_dec n1 n2) as [<-|ne]; [left|right]; cbn in H; destruct H as [<- ->]; [reflexivity|intros [=f]; exact (ne f)].
   - intros e2; destruct (exp_inv e2) as [ [ [ [ [
-      (c' & ->) | (b' & eq1 & ->) ] | (b' & eq1 & ->) ] | (tin & op & e1' & ->) ] | (ty1 & ty2 & op & e1' & e2' & ->) ] | (eb & et & ef & ->) ].
-    2: right; destruct b, b'; cbn in eq1; subst; discriminate.
+      (c' & ->) | (b' & H) ] | (b' & H) ] | (tin & op & e1' & ->) ] | (ty1 & ty2 & op & e1' & e2' & ->) ] | (eb & et & ef & ->) ].
+    2: right; destruct H as [eq1 ->]; destruct b, b'; cbn in eq1; subst; discriminate.
     1,3-5: right; subst; discriminate.
-    destruct b as [n1 ty1], b' as [n2 ty2]; cbn in eq1; subst ty2.
-    destruct (PeanoNat.Nat.eq_dec n1 n2) as [<-|ne]; [left; reflexivity|right; cbn; intros [=f]; exact (ne f)].
+    destruct b as [n1 ty1], b' as [n2 ty2].
+    destruct (PeanoNat.Nat.eq_dec n1 n2) as [<-|ne]; [left|right]; cbn in H; destruct H as [<- ->]; [reflexivity|intros [=f]; exact (ne f)].
   - intros e2; destruct (exp_inv e2) as [ [ [ [ [
-      (c' & ->) | (b' & eq1 & ->) ] | (b' & eq1 & ->) ] | (tin' & op' & e1' & ->) ] | (ty1 & ty2 & op' & e1' & e2' & ->) ] | (eb & et & ef & ->) ].
-    1-3,5-6: right; subst; discriminate.
+      (c' & ->) | (b' & H) ] | (b' & H) ] | (tin' & op' & e1' & ->) ] | (ty1 & ty2 & op' & e1' & e2' & ->) ] | (eb & et & ef & ->) ].
+    1-3,5-6: right; try destruct H as [eq1 ->]; subst; discriminate.
     destruct (type_dec tin tin') as [<-|ne]; [|right; intros [=f _ _]; exact (ne f)].
     destruct (unop_dec op op') as [<-|ne]; [|right; intros [=f _]; exact (ne (sig2T_eq_type (sig2T_eq_type f)))].
     destruct (IH e1') as [<-|ne]; [|right; intros [=f]; exact (ne (sig2T_eq_type f))].
     left; reflexivity.
   - intros e2; destruct (exp_inv e2) as [ [ [ [ [
-      (c' & ->) | (b' & eq1 & ->) ] | (b' & eq1 & ->) ] | (tin' & op' & e1' & ->) ] | (ty1' & ty2' & op' & e1' & e2' & ->) ] | (eb & et & ef & ->) ].
-    1-4,6: right; subst; discriminate.
+      (c' & ->) | (b' & H) ] | (b' & H) ] | (tin' & op' & e1' & ->) ] | (ty1' & ty2' & op' & e1' & e2' & ->) ] | (eb & et & ef & ->) ].
+    1-4,6: right; try destruct H as [eq1 ->]; subst; discriminate.
     destruct (type_dec ty1 ty1') as [<-|ne]; [|right; intros [=f _ _ _]; exact (ne f)].
     destruct (type_dec ty2 ty2') as [<-|ne]; [|right; intros [=f _ _]; exact (ne f)].
     destruct (binop_dec op op') as [<-|ne]; [|right; intros [=f _]; exact (ne (sig2T_eq_type (sig2T_eq_type (sig2T_eq_type f))))].
@@ -308,8 +311,8 @@ Proof.
     destruct (IH2 e2') as [<-|ne]; [|right; intros [=f]; exact (ne (sig2T_eq_type f))].
     left; reflexivity.
   - intros e2; destruct (exp_inv e2) as [ [ [ [ [
-      (c' & ->) | (b' & eq1 & ->) ] | (b' & eq1 & ->) ] | (tin' & op' & e1' & ->) ] | (ty1' & ty2' & op' & e1' & e2' & ->) ] | (eb2 & et2 & ef2 & ->) ].
-    1-5: right; subst; discriminate.
+      (c' & ->) | (b' & H) ] | (b' & H) ] | (tin' & op' & e1' & ->) ] | (ty1' & ty2' & op' & e1' & e2' & ->) ] | (eb2 & et2 & ef2 & ->) ].
+    1-5: right; try destruct H as [eq1 ->]; subst; discriminate.
     destruct (IHb eb2) as [<-|ne]; [|right; intros [=f]; exact (ne f)].
     destruct (IHt et2) as [<-|ne]; [|right; intros [=f]; exact (ne (sig2T_eq_type f))].
     destruct (IHf ef2) as [<-|ne]; [|right; intros [=f]; exact (ne (sig2T_eq_type f))].
@@ -347,10 +350,10 @@ Record node := mk_node {
   n_body: list equation;
 
   n_vars: list binder := n_in ++ n_out :: n_locals;
-  n_assigned_vars: list ident := map fst n_body;
+  n_assigned_vars: list binder := map (fun '(n, existT _ ty _) => (n, ty)) n_body;
 
-  n_assigned_vars_are_vars: incl n_assigned_vars (map fst n_vars);
-  n_assigned_out: In (fst n_out) n_assigned_vars;
+  n_assigned_vars_are_vars: incl n_assigned_vars n_vars;
+  n_assigned_out: In n_out n_assigned_vars;
   n_out_is_not_an_input: ~ In (fst n_out) (map fst n_in);
   n_inputs_equations: incl (List.map (fun '((n, ty) as b) => (n, existT exp ty (EInput b))) n_in) n_body;
   n_no_einputs_in_other: Forall (fun '(name, existT _ ty exp) => ~ In name (map fst n_in) -> has_einput exp = false) n_body;
@@ -373,6 +376,60 @@ Inductive value : type -> Set :=
   | VBinop : forall {ty1 ty2 tout}, binop ty1 ty2 tout -> value ty1 -> value ty2 -> value tout
   | VIfte  : forall {ty}, value TBool -> value ty -> value ty -> value ty
 .
+
+Lemma value_inv {ty} (x: value ty) :
+  {c : const ty | x = VConst c} +
+  {b | exists (eq : ty = _), x = eq_rect _ value (VInput b) _ (eq_sym eq)} +
+  {tin : type & {op : unop tin ty & {e : value tin | x = VUnop op e}}} +
+  {ty1 : type & {ty2 : type & {op : binop ty1 ty2 ty & {e1 : value ty1 & {e2 : value ty2 | x = VBinop op e1 e2}}}}} +
+  {eb : value TBool & {et : value ty & {ef : value ty | x = VIfte eb et ef}}}.
+Proof using.
+  destruct x.
+  1-4: left.
+  1-3: left.
+  1-2: left.
+  1-1: left.
+  2-5: right.
+  all: try solve [repeat eexists; exact eq_refl].
+  exists b, eq_refl; exact eq_refl.
+Qed.
+Lemma value_dec {ty} (e1 e2: value ty) : {e1 = e2} + {e1 <> e2}.
+Proof.
+  revert e2.
+  induction e1 as [ ty c | b | tin tout op e1 IH | ty1 ty2 tout op e11 IH1 e12 IH2 | ty eb1 IHb et1 IHt ef1 IHf ].
+  - intros e2; destruct (value_inv e2) as [ [ [ [
+      (c' & ->) | (b' & H) ] | (tin & op & e1' & ->) ] | (ty1 & ty2 & op & e1' & e2' & ->) ] | (eb & et & ef & ->) ].
+    1: destruct (const_dec c c') as [e|n]; [left; exact (f_equal _ e)|right; intros [=f]; apply sig2T_eq_type in f; exact (n f)].
+    all: right; try destruct H as [eq1 ->]; subst; discriminate.
+  - intros e2; destruct (value_inv e2) as [ [ [ [
+      (c' & ->) | (b' & H) ] | (tin & op & e1' & ->) ] | (ty1 & ty2 & op & e1' & e2' & ->) ] | (eb & et & ef & ->) ].
+    1,3-5: right; subst; discriminate.
+    destruct b as [n1 ty1], b' as [n2 ty2].
+    destruct (PeanoNat.Nat.eq_dec n1 n2) as [<-|ne]; [left|right]; cbn in H; destruct H as [<- ->]; [reflexivity|intros [=f]; exact (ne f)].
+  - intros e2; destruct (value_inv e2) as [ [ [ [
+      (c' & ->) | (b' & H) ] | (tin' & op' & e1' & ->) ] | (ty1 & ty2 & op' & e1' & e2' & ->) ] | (eb & et & ef & ->) ].
+    1-2,4-5: right; try destruct H as [eq1 ->]; subst; discriminate.
+    destruct (type_dec tin tin') as [<-|ne]; [|right; intros [=f _ _]; exact (ne f)].
+    destruct (unop_dec op op') as [<-|ne]; [|right; intros [=f _]; exact (ne (sig2T_eq_type (sig2T_eq_type f)))].
+    destruct (IH e1') as [<-|ne]; [|right; intros [=f]; exact (ne (sig2T_eq_type f))].
+    left; reflexivity.
+  - intros e2; destruct (value_inv e2) as [ [ [ [
+      (c' & ->) | (b' & H) ] | (tin' & op' & e1' & ->) ] | (ty1' & ty2' & op' & e1' & e2' & ->) ] | (eb & et & ef & ->) ].
+    1-3,5: right; try destruct H as [eq1 ->]; subst; discriminate.
+    destruct (type_dec ty1 ty1') as [<-|ne]; [|right; intros [=f _ _ _]; exact (ne f)].
+    destruct (type_dec ty2 ty2') as [<-|ne]; [|right; intros [=f _ _]; exact (ne f)].
+    destruct (binop_dec op op') as [<-|ne]; [|right; intros [=f _]; exact (ne (sig2T_eq_type (sig2T_eq_type (sig2T_eq_type f))))].
+    destruct (IH1 e1') as [<-|ne]; [|right; intros [=f]; exact (ne (sig2T_eq_type f))].
+    destruct (IH2 e2') as [<-|ne]; [|right; intros [=f]; exact (ne (sig2T_eq_type f))].
+    left; reflexivity.
+  - intros e2; destruct (value_inv e2) as [ [ [ [
+      (c' & ->) | (b' & H) ] | (tin' & op' & e1' & ->) ] | (ty1' & ty2' & op' & e1' & e2' & ->) ] | (eb2 & et2 & ef2 & ->) ].
+    1-4: right; try destruct H as [eq1 ->]; subst; discriminate.
+    destruct (IHb eb2) as [<-|ne]; [|right; intros [=f]; exact (ne f)].
+    destruct (IHt et2) as [<-|ne]; [|right; intros [=f]; exact (ne (sig2T_eq_type f))].
+    destruct (IHf ef2) as [<-|ne]; [|right; intros [=f]; exact (ne (sig2T_eq_type f))].
+    left; reflexivity.
+Qed.
 
 Definition history := Dict.t {ty & Stream.t (value ty)}.
 Definition in_history (h : history) '((v, ty) : nat * type) := match Dict.find v h with
